Try my hand at a compatibility lemma. Suggests some minor changes in the infrastructure.

Compiler/Erase.v
@@ -4,59 +4,67 @@ Require Import Stlc.SpecTyping.
 Require Import Stlc.LemmasTyping.
 Require Import Utlc.SpecScoping.
 Require Import Utlc.LemmasScoping.
+Require Import LogRel.PseudoType.
+Require Import LogRel.LR.
+Require Import LogRel.LemmasLR.
 Require Utlc.Fix.
 
-Module SS := Stlc.SpecSyntax.
-Module US := Utlc.SpecSyntax.
-Module UF := Utlc.Fix.
+Module S.
+    Include Stlc.SpecSyntax.
+    Include Stlc.LemmasTyping.
+End S.
+Module U.
+  Include Utlc.SpecSyntax.
+  Include Utlc.Fix.
+End U.
 
-Fixpoint erase (t : SS.Tm) : US.UTm :=
+Fixpoint erase (t : S.Tm) : U.UTm :=
   match t with
-    | SS.abs τ t         => US.abs (erase t)
-    | SS.unit            => US.unit
-    | SS.true            => US.true
-    | SS.false           => US.false
-    | SS.pair t₁ t₂      => US.pair (erase t₁) (erase t₂)
-    | SS.inl t           => US.inl (erase t)
-    | SS.inr t           => US.inr (erase t)
-    | SS.var x           => US.var x
-    | SS.app t₁ t₂       => US.app (erase t₁) (erase t₂)
-    | SS.ite t₁ t₂ t₃    => US.ite (erase t₁) (erase t₂) (erase t₃)
-    | SS.proj₁ t₁        => US.proj₁ (erase t₁)
-    | SS.proj₂ t₁        => US.proj₂ (erase t₁)
-    | SS.caseof t₁ t₂ t₃ => US.caseof (erase t₁) (erase t₂) (erase t₃)
-    | SS.seq t₁ t₂       => US.seq (erase t₁) (erase t₂)
-    | SS.fixt _ _ t₁     => US.app UF.ufix (erase t₁)
+    | S.abs τ t         => U.abs (erase t)
+    | S.unit            => U.unit
+    | S.true            => U.true
+    | S.false           => U.false
+    | S.pair t₁ t₂      => U.pair (erase t₁) (erase t₂)
+    | S.inl t           => U.inl (erase t)
+    | S.inr t           => U.inr (erase t)
+    | S.var x           => U.var x
+    | S.app t₁ t₂       => U.app (erase t₁) (erase t₂)
+    | S.ite t₁ t₂ t₃    => U.ite (erase t₁) (erase t₂) (erase t₃)
+    | S.proj₁ t₁        => U.proj₁ (erase t₁)
+    | S.proj₂ t₁        => U.proj₂ (erase t₁)
+    | S.caseof t₁ t₂ t₃ => U.caseof (erase t₁) (erase t₂) (erase t₃)
+    | S.seq t₁ t₂       => U.seq (erase t₁) (erase t₂)
+    | S.fixt _ _ t₁     => U.app U.ufix (erase t₁)
   end.
 
-Fixpoint erase_pctx (C : SS.PCtx) : US.PCtx :=
+Fixpoint erase_pctx (C : S.PCtx) : U.PCtx :=
   match C with
-    | SS.phole => phole
-    | SS.pabs τ C => US.pabs (erase_pctx C)
-    | SS.papp₁ C t => US.papp₁ (erase_pctx C) (erase t) 
-    | SS.papp₂ t C => US.papp₂ (erase t) (erase_pctx C)
-    | SS.pite₁ C t₂ t₃ => US.pite₁ (erase_pctx C) (erase t₂) (erase t₃)
-    | SS.pite₂ t₁ C t₃ => US.pite₂ (erase t₁) (erase_pctx C) (erase t₃)
-    | SS.pite₃ t₁ t₂ C => US.pite₃ (erase t₁) (erase t₂) (erase_pctx C)
-    | SS.ppair₁ C t => US.ppair₁ (erase_pctx C) (erase t)
-    | SS.ppair₂ t C => US.ppair₂ (erase t) (erase_pctx C)
-    | SS.pproj₁ C => US.pproj₁ (erase_pctx C)
-    | SS.pproj₂ C => US.pproj₂ (erase_pctx C)
-    | SS.pinl C => US.pinl (erase_pctx C)
-    | SS.pinr C => US.pinr (erase_pctx C)
-    | SS.pcaseof₁ C t₂ t₃ => US.pcaseof₁ (erase_pctx C) (erase t₂) (erase t₃)
-    | SS.pcaseof₂ t₁ C t₃ => US.pcaseof₂ (erase t₁) (erase_pctx C) (erase t₃)
-    | SS.pcaseof₃ t₁ t₂ C => US.pcaseof₃ (erase t₁) (erase t₂) (erase_pctx C)
-    | SS.pseq₁ C t => US.pseq₁ (erase_pctx C) (erase t)
-    | SS.pseq₂ t C => US.pseq₂ (erase t) (erase_pctx C)
-    | SS.pfixt τ₁ τ₂ C => US.papp₂ UF.ufix (erase_pctx C)
+    | S.phole => phole
+    | S.pabs τ C => U.pabs (erase_pctx C)
+    | S.papp₁ C t => U.papp₁ (erase_pctx C) (erase t) 
+    | S.papp₂ t C => U.papp₂ (erase t) (erase_pctx C)
+    | S.pite₁ C t₂ t₃ => U.pite₁ (erase_pctx C) (erase t₂) (erase t₃)
+    | S.pite₂ t₁ C t₃ => U.pite₂ (erase t₁) (erase_pctx C) (erase t₃)
+    | S.pite₃ t₁ t₂ C => U.pite₃ (erase t₁) (erase t₂) (erase_pctx C)
+    | S.ppair₁ C t => U.ppair₁ (erase_pctx C) (erase t)
+    | S.ppair₂ t C => U.ppair₂ (erase t) (erase_pctx C)
+    | S.pproj₁ C => U.pproj₁ (erase_pctx C)
+    | S.pproj₂ C => U.pproj₂ (erase_pctx C)
+    | S.pinl C => U.pinl (erase_pctx C)
+    | S.pinr C => U.pinr (erase_pctx C)
+    | S.pcaseof₁ C t₂ t₃ => U.pcaseof₁ (erase_pctx C) (erase t₂) (erase t₃)
+    | S.pcaseof₂ t₁ C t₃ => U.pcaseof₂ (erase t₁) (erase_pctx C) (erase t₃)
+    | S.pcaseof₃ t₁ t₂ C => U.pcaseof₃ (erase t₁) (erase t₂) (erase_pctx C)
+    | S.pseq₁ C t => U.pseq₁ (erase_pctx C) (erase t)
+    | S.pseq₂ t C => U.pseq₂ (erase t) (erase_pctx C)
+    | S.pfixt τ₁ τ₂ C => U.papp₂ U.ufix (erase_pctx C)
   end.
 
-Lemma erase_scope (t : SS.Tm) (Γ : SS.Env) (τ : SS.Ty) :
+Lemma erase_scope (t : S.Tm) (Γ : S.Env) (τ : S.Ty) :
   ⟪ Γ ⊢ t : τ ⟫ -> ⟨ dom Γ ⊢ erase t ⟩.
 Proof.
   intro wt; induction wt; crushUtlcScoping.
-  apply UF.ufix_ws.
+  apply U.ufix_ws.
 Qed.
 
 Hint Extern 4 ⟨ _ ⊢ erase ?t ⟩ =>
@@ -64,9 +72,41 @@ Hint Extern 4 ⟨ _ ⊢ erase ?t ⟩ =>
       [ H : ⟪ _ ⊢ ?t : _ ⟫ |- _ ] => refine (erase_scope _ _ _ H)
   end.
 
-Lemma erase_pctx_scope (C : SS.PCtx) (Γ₀ Γ : SS.Env) (τ₀ τ : SS.Ty) :
+Lemma erase_pctx_scope (C : S.PCtx) (Γ₀ Γ : S.Env) (τ₀ τ : S.Ty) :
   ⟪ ⊢ C : Γ₀ , τ₀ → Γ , τ ⟫ → ⟨ ⊢ erase_pctx C : dom Γ₀ → dom Γ ⟩.
 Proof.
   intro wt; induction wt; crushUtlcScoping.
-  apply UF.ufix_ws.
+  apply U.ufix_ws.
 Qed.
+
+(* Domi: it would be more convenient to define envrel similar to WtSub using
+   something like GetEVar. Perhaps generalize GetEVar *)
+(* Lemma envrel_implies_WtSub {d W Γ γs γu} : *)
+(*   envrel d W Γ γs γu → WtSub (repEmulCtx Γ) empty γs. *)
+(* Proof. *)
+(*   Print WtSub. *)
+(*   intros envrel i τ vi_τ. *)
+(*   Print envrel. *)
+
+
+(* Section CompatibilityLemmas. *)
+(*   Lemma compat_lambda {Γ τ' ts d n tu τ} : *)
+(*     ⟪ Γ p▻ τ' ⊩ ts ⟦ d , n ⟧ tu : τ ⟫ → *)
+(*     ⟪ Γ ⊩ (S.abs (repEmul τ') ts) ⟦ d , n ⟧ abs tu : ptarr τ' τ ⟫. *)
+(*   Proof. *)
+(*     intros lr. *)
+(*     unfold OpenLRN in *. *)
+(*     destruct_conjs. *)
+(*     split; crushTyping. *)
+(*     apply valrel_in_termrel. *)
+(*     unfold valrel, valrel'. *)
+(*     unfold well_founded_induction_type, Acc_rect. *)
+(*     unfold valrel'' in |- *. *)
+(*     simpl. *)
+(*     split. *)
+(*     -  unfold OfType, OfTypeStlc, OfTypeUtlc; split. *)
+(*        + replace (S.abs (repEmul τ') (ts [γs↑])) with ((S.abs (repEmul τ') ts) [γs]). *)
+(*          refine (S.typing_sub _ _ _ _); crushTyping. *)
+         
+
+(* End CompabilityLemmas. *)
